Checkpoint

Orderedtree/DOrderedTree/Internal/Cell.lean
@@ -15,68 +15,68 @@ variable {α : Type u} {β : α → Type v} {γ : α → Type w} {δ : Type w}
 namespace Std.DOrderedTree.Internal
 
 /-- Type for representing the place in a binary search tree where a mapping for `k` could live. -/
-structure Cell (α : Type u) [Ord α] (β : α → Type v) (k : α) where
+structure Cell (α : Type u) [Ord α] (β : α → Type v) (k : α → Ordering) where
   /-- The mapping. -/
   inner : Option ((a : α) × β a)
   /-- If there is a mapping, then it has a matching key. -/
-  property : ∀ [OrientedOrd α], ∀ p, inner = some p → compare k p.1 = .eq
+  property : ∀ [OrientedOrd α], ∀ p, inner = some p → k p.1 = .eq
 
 namespace Cell
 
 /-- Create a cell with a matching key. -/
-def ofEq [Ord α] {k : α} (k' : α) (v' : β k') (hcmp : ∀ [OrientedOrd α], compare k k' = .eq) :
+def ofEq [Ord α] {k : α → Ordering} (k' : α) (v' : β k') (hcmp : ∀ [OrientedOrd α], k k' = .eq) :
     Cell α β k :=
   ⟨some ⟨k', v'⟩, by intro _ p hp; obtain rfl := Option.some_inj.1 hp; simpa using hcmp⟩
 
 /-- Create a cell with a matching key. -/
-def of [Ord α] (k : α) (v : β k) : Cell α β k :=
+def of [Ord α] (k : α) (v : β k) : Cell α β (compare k) :=
   .ofEq k v (by intro; simp)
 
 @[simp] theorem ofEq_inner [Ord α] {k k' : α} {v' : β k'} {h} :
-  (Cell.ofEq k' v' h : Cell α β k).inner = some ⟨k', v'⟩ := rfl
+  (Cell.ofEq k' v' h : Cell α β (compare k)).inner = some ⟨k', v'⟩ := rfl
 @[simp] theorem of_inner [Ord α] {k : α} {v : β k} : (Cell.of k v).inner = some ⟨k, v⟩ := rfl
 
 /-- Create an empty cell. -/
-def empty [Ord α] {k : α} : Cell α β k :=
+def empty [Ord α] {k : α → Ordering} : Cell α β k :=
   ⟨none, by simp⟩
 
-@[simp] theorem empty_inner [Ord α] {k : α} : (Cell.empty : Cell α β k).inner = none := rfl
+@[simp] theorem empty_inner [Ord α] {k : α} : (Cell.empty : Cell α β (compare k)).inner = none := rfl
 
-def contains [Ord α] {k : α} (c : Cell α β k) : Bool :=
+def contains [Ord α] {k : α → Ordering} (c : Cell α β k) : Bool :=
   c.inner.isSome
 
 @[simp] theorem contains_of [Ord α] {k : α} {v : β k} : (Cell.of k v).contains = true := rfl
-@[simp] theorem contains_ofEq [Ord α] {k k' : α} {v' : β k'} {h} :
+@[simp] theorem contains_ofEq [Ord α] {k : α → Ordering} {k' : α} {v' : β k'} {h} :
     (Cell.ofEq k' v' h : Cell α β k).contains = true := rfl
-@[simp] theorem contains_empty [Ord α] {k : α} : (Cell.empty : Cell α β k).contains = false := rfl
+@[simp] theorem contains_empty [Ord α] {k : α → Ordering} : (Cell.empty : Cell α β k).contains = false := rfl
 
-def get? [Ord α] [OrientedOrd α] [LawfulEqOrd α] {k : α} (c : Cell α β k) : Option (β k) :=
+def get? [Ord α] [OrientedOrd α] [LawfulEqOrd α] {k : α} (c : Cell α β (compare k)) : Option (β k) :=
   match h : c.inner with
   | none => none
   | some p => some (cast (congrArg β (eq_of_compare (c.property _ h)).symm) p.2)
 
 @[simp]
 theorem get?_empty [Ord α] [OrientedOrd α] [LawfulEqOrd α] {k : α} :
-    (Cell.empty : Cell α β k).get? = none :=
+    (Cell.empty : Cell α β (compare k)).get? = none :=
   rfl
 
-def get [Ord α] [OrientedOrd α] [LawfulEqOrd α] {k : α} (c : Cell α β k) (h : c.contains) : β k :=
+def get [Ord α] [OrientedOrd α] [LawfulEqOrd α] {k : α} (c : Cell α β (compare k)) (h : c.contains) : β k :=
   match hc : c.inner with
   | none => False.elim (by simp [contains, hc] at h)
   | some p => (cast (congrArg β (eq_of_compare (c.property _ hc)).symm) p.2)
 
-theorem ext [Ord α] {k : α} {c c' : Cell α β k} : c.inner = c'.inner → c = c' := by
+theorem ext [Ord α] {k : α} {c c' : Cell α β (compare k)} : c.inner = c'.inner → c = c' := by
   cases c; cases c'; simp
 
 end Cell
 
-def List.findCell [Ord α] (l : List ((a : α) × β a)) (k : α) : Cell α β k where
-  inner := l.find? (compare k ·.1 == .eq)
+def List.findCell [Ord α] (l : List ((a : α) × β a)) (k : α → Ordering) : Cell α β k where
+  inner := l.find? (k ·.1 == .eq)
   property p hp := by simpa using (List.find?_eq_some_iff_append.1 hp).1
 
-theorem List.findCell_inner [Ord α] (l : List ((a : α) × β a)) (k : α) :
-    (findCell l k).inner = l.find? (compare k ·.1 == .eq) := rfl
+theorem List.findCell_inner [Ord α] (l : List ((a : α) × β a)) (k : α → Ordering) :
+    (findCell l k).inner = l.find? (k ·.1 == .eq) := rfl
 
-@[simp] theorem List.findCell_nil [Ord α] (k : α) : (findCell [] k : Cell α β k) = .empty := rfl
+@[simp] theorem List.findCell_nil [Ord α] (k : α → Ordering) : (findCell [] k : Cell α β k) = .empty := rfl
 
 end Std.DOrderedTree.Internal
