Orderedtree/DOrderedTree/Internal/Impl.lean
@@ -165,6 +165,22 @@ where
     | .eq => some ⟨ky, y⟩
     | .gt => go best r
 
+/-- The smallest element of `l` that is greater than `k`. -/
+def upperBound? [Ord α] (k : α) : Impl α β → Option ((a : α) × β a) :=
+  go none
+where
+  go (best : Option ((a : α) × β a)) : Impl α β → Option ((a : α) × β a)
+  | .leaf => best
+  | .inner _ ky y l r => match compare k ky with
+    | .lt => go (some ⟨ky, y⟩) l
+    | _ => go best r
+
+/-- The smallest element of `l`. -/
+def min? [Ord α] : Impl α β → Option ((a : α) × β a)
+  | .leaf => none
+  | .inner _ k v .leaf _ => some ⟨k, v⟩
+  | .inner _ _ _ l@(.inner _ _ _ _ _) _ => l.min?
+
 /-- Predicate for local balance at a node of the tree. We don't provide API for this, preferring
 instead to use automation to dispatch goals about balance. -/
 @[tree_tac]
